task 3

hw3.thy
@@ -1,12 +1,12 @@
 theory hw3
   imports  
   "HOL-Library.Countable_Set"
-  abbrevs "|=0" = "⊨⇩∅" and "||=0" = "⊫⇩∅" and ",," = "⇩♭"
+  abbrevs "|=0" = "\<Turnstile>\<^sub>\<emptyset>" and "||=0" = "\<TTurnstile>\<^sub>\<emptyset>" and ",," = "\<^sub>\<flat>"
 begin
 (*1*)
 datatype exp = Var | Const int | Add exp exp | Mult exp exp
 
-fun eval :: "exp ⇒ int ⇒ int" where
+fun eval :: "exp \<Rightarrow> int \<Rightarrow> int" where
   "eval Var v = v" |
   "eval (Const e) v = e" |
   "eval (Add e f) v = (eval e v) + (eval f v)" |
@@ -14,12 +14,12 @@ fun eval :: "exp ⇒ int ⇒ int" where
 
 value "eval (Var) 6"
 
-fun evalp :: "int list ⇒ int ⇒ int" where
+fun evalp :: "int list \<Rightarrow> int \<Rightarrow> int" where
   "evalp Nil v = 0" |
   "evalp (Cons x xs) v = x + v * (evalp xs v)"
 
 value "evalp [4, 2, -1, 3] 4"
-fun add_coeff :: "int list ⇒ int list ⇒ int list" where
+fun add_coeff :: "int list \<Rightarrow> int list \<Rightarrow> int list" where
   "add_coeff Nil Nil = Nil" |
   "add_coeff Nil ys = ys" |
   "add_coeff xs Nil = xs" |
@@ -32,7 +32,7 @@ lemma evalp_add[simp] : "evalp (add_coeff xs ys) x = (evalp xs x) + (evalp ys x)
      apply(auto simp add: algebra_simps)
   done
 
-fun mult :: "int ⇒ int list ⇒ int list" where
+fun mult :: "int \<Rightarrow> int list \<Rightarrow> int list" where
   "mult n Nil = Nil" |
   "mult n (x#xs) = (n*x)#(mult n xs)"
 
@@ -41,7 +41,7 @@ lemma evalp_mul[simp] : "evalp (mult n xs) v = n * (evalp xs v)"
    apply(auto simp add:algebra_simps)
   done
 
-fun mult_coeff :: "int list ⇒ int list ⇒ int list" where
+fun mult_coeff :: "int list \<Rightarrow> int list \<Rightarrow> int list" where
   "mult_coeff Nil ys = Nil" |
   "mult_coeff (x#xs) ys = add_coeff (mult x ys) (0#(mult_coeff xs ys))"
 
@@ -50,7 +50,7 @@ lemma evalp_mult[simp] : "evalp (mult_coeff xs ys) x = (evalp xs x) * (evalp ys 
    apply(auto simp add: algebra_simps)
   done
 
-fun coeff :: "exp ⇒ int list" where
+fun coeff :: "exp \<Rightarrow> int list" where
 "coeff Var = [0,1]" |
 "coeff (Const i) = [i]" |
 "coeff (Add e f) = add_coeff (coeff e) (coeff f)" |
@@ -66,22 +66,83 @@ theorem preservation : "evalp (coeff e) x = eval e x"
 
 (*2*)
 
-abbreviation vx ("❙x") where "❙x ≡ Var"
-abbreviation add (infixl "❙+" 65) where "a ❙+ b ≡ Add a b"
-abbreviation mul (infixl "❙×" 70) where "a ❙× b ≡ Mult a b"
-abbreviation num ("❙_" [1000] 1000) where "❙a ≡ Const a"
+abbreviation vx ("\<^bold>x") where "\<^bold>x \<equiv> Var"
+abbreviation add (infixl "\<^bold>+" 65) where "a \<^bold>+ b \<equiv> Add a b"
+abbreviation mul (infixl "\<^bold>\<times>" 70) where "a \<^bold>\<times> b \<equiv> Mult a b"
+abbreviation num ("\<^bold>_" [1000] 1000) where "\<^bold>a \<equiv> Const a"
 
-no_notation  power2  ("(_⇧2)" [1000] 999)
+no_notation  power2  ("(_\<^sup>2)" [1000] 999)
 
-primrec pow :: "exp ⇒ nat ⇒ exp" ("_⇧_" [1000, 1000] 80)  
+primrec pow :: "exp \<Rightarrow> nat \<Rightarrow> exp" ("_\<^sup>_" [1000, 1000] 80)  
   where
-  "pow x 0       = ❙1"
-| "pow x (Suc n) = x ❙× (pow x n)"
+  "pow x 0       = \<^bold>1"
+| "pow x (Suc n) = x \<^bold>\<times> (pow x n)"
 
-value "eval( ❙4 ❙+ ❙2❙×❙x⇧3 ❙+ ❙(-1) ❙× ❙x⇧2 ❙+ ❙3❙×❙x⇧3) 3"
+value "eval( \<^bold>4 \<^bold>+ \<^bold>2\<^bold>\<times>\<^bold>x\<^sup>3 \<^bold>+ \<^bold>(-1) \<^bold>\<times> \<^bold>x\<^sup>2 \<^bold>+ \<^bold>3\<^bold>\<times>\<^bold>x\<^sup>3) 3"
 
 (*3*)
-          
+datatype boolex = Const bool | Var nat | Neg boolex | And boolex boolex
+
+primrec "value" :: "boolex \<Rightarrow> (nat \<Rightarrow> bool) \<Rightarrow> bool" where
+"value (Const b) env = b" |
+"value (Var x) env = env x" |
+"value (Neg b) env = (\<not> value b env)" |
+"value (And b c) env = (value b env \<and> value c env)"
+
+datatype ifex = CIF bool | VIF nat | IF ifex ifex ifex
+
+primrec valif :: "ifex \<Rightarrow> (nat \<Rightarrow> bool) \<Rightarrow> bool" where
+"valif (CIF b) env = b" |
+"valif (VIF x) env = env x" |
+"valif (IF b t e) env = (if valif b env then valif t env else valif e env)"
+
+primrec bool2if :: "boolex \<Rightarrow> ifex" where
+"bool2if (Const b) = CIF b" |
+"bool2if (Var x) = VIF x" |
+"bool2if (Neg b) = IF (bool2if b) (CIF False) (CIF True)" |
+"bool2if (And b c) = IF (bool2if b) (bool2if c) (CIF False)"
+
+lemma "valif (bool2if b) env = value b env"
+  apply(induct_tac b)
+  apply(auto)
+  done
+
 (*4*)
+locale Geom =
+  fixes on :: "'p \<Rightarrow> 'l \<Rightarrow> bool"
+  assumes line_on_two_pts: "a \<noteq> b \<Longrightarrow> \<exists>l. on a l \<and> on b l" 
+  and line_on_two_pts_unique: 
+  "\<lbrakk> a \<noteq> b; on a l; on b l; on a m; on b m \<rbrakk> \<Longrightarrow> l = m"
+  and two_points_on_line: "\<exists>a b. a \<noteq> b \<and> on a l \<and> on b l"
+  and three_points_not_on_line: "\<exists>a b c. a \<noteq> b \<and> a \<noteq> c \<and> b \<noteq> c \<and> \<not> (\<exists>l. on a l \<and> on b l \<and> on c l)"
+begin
+  
+
+lemma three_points_not_on_line_alt:
+  "\<exists>a b c. a \<noteq> b \<and> a \<noteq> c \<and> b \<noteq> c \<and> (\<forall>l. on a l \<and> on b l \<longrightarrow> \<not> on c l)"
+proof -
+  obtain a b c 
+    where distinct: "a \<noteq> b \<and> a \<noteq> c \<and> b \<noteq> c" 
+                    "\<not> (\<exists>l. on a l \<and> on b l \<and> on c l)" 
+    using three_points_not_on_line by blast
+  then have "\<forall>l. on a l \<and> on b l \<longrightarrow> \<not> on c l"
+    by blast
+  thus ?thesis using distinct by blast
+qed        
+  
+lemma exists_pt_not_on_line: "\<exists>x. \<not> on x l"
+proof -
+   obtain a b c where l3: "\<not> (on a l \<and> on b l \<and> on c l)" using three_points_not_on_line by blast 
+   thus ?thesis by blast 
+ qed
+
+(*lemma two_lines_unique_intersect_pt:
+  assumes l m: "l\<noteq>m and on x l and on x m and on y l and on y m shows x=y"
+proof(rule ccontr)
+  assumes "x\<noteq>y" then have "l=m" using line_on_two_pts_unique assms by simp
+  thus False using lm by simp
+qed*)
+
+end
 
 end
